up

lambda/coq/lambda.v
@@ -36,24 +36,6 @@ Definition subst := subst_rec 0.
 
 Notation "t '[' x '<-' u ']'" := (subst t u x) (at level 20).
 
-(* star reduction *)
-
-Inductive star (R : lambda -> lambda -> Prop) : lambda -> lambda -> Prop :=
-  | refl : forall M, star R M M
-  | step : forall M M' N, R M M' -> star R M' N -> star R M N
-.
-
-(* Beta-reduction *)
-
-Inductive b_red : lambda -> lambda -> Prop :=
-  | beta    : forall M N, b_red (App (Abs M) N) (subst M N 0)
-  | b_abs   : forall M M', b_red M M' -> b_red (Abs M) (Abs M')
-  | b_app1  : forall M M' N, b_red M M' -> b_red (App M N) (App M' N)
-  | b_app2  : forall M N N', b_red N N' -> b_red (App M N) (App M N')
-.
-
-Definition b_star := star b_red.
-
 (* free *)
 Fixpoint free_rec n' (L : lambda) n :=
   match L with
@@ -199,4 +181,70 @@ Proof.
   unfold subst.
   now apply comm_subst_rec.
 Qed.
+
+(* star reduction *)
+
+Inductive star (R : lambda -> lambda -> Prop) : lambda -> lambda -> Prop :=
+  | refl : forall M, star R M M
+  | step : forall M M' N, R M M' -> star R M' N -> star R M N
+.
+
+(* Beta-reduction *)
+
+Inductive b_red : lambda -> lambda -> Prop :=
+  | beta    : forall M N, b_red (App (Abs M) N) (subst M N 0)
+  | b_abs   : forall M M', b_red M M' -> b_red (Abs M) (Abs M')
+  | b_app1  : forall M M' N, b_red M M' -> b_red (App M N) (App M' N)
+  | b_app2  : forall M N N', b_red N N' -> b_red (App M N) (App M N')
+.
+
+Definition b_star := star b_red.
+
+(* parralel reduction *)
+
+Inductive b_parr: lambda -> lambda -> Prop :=
+  | refl_p   : forall x, b_parr (Var x) (Var x)
+  | betap    : forall M N M' N',
+      b_parr M M' -> b_parr N N' ->
+      b_parr (App (Abs M) N) (subst M' N' 0)
+  | bp_abs   : forall M M', b_parr M M' -> b_parr (Abs M) (Abs M')
+  | bp_app   : forall M M' N N',
+      b_parr M M' -> b_parr N N' ->
+      b_parr (App M N) (App M' N')
+.
+
+Lemma par_refl:
+  forall T,
+  b_parr T T.
+Proof.
+  induction T.
+  - constructor.
+  - constructor. apply IHT.
+  - eapply bp_app; auto.
+Qed.
+
+Lemma b_to_par:
+  forall T T',
+  b_red T T' -> b_parr T T'.
+Proof.
+  intros T T' H. induction H.
+  - constructor; apply par_refl.
+  - constructor. apply IHb_red. 
+  - econstructor. apply IHb_red.
+    apply par_refl.
+  - eapply bp_app. apply par_refl.
+    apply IHb_red.
+Qed.
+
+Lemma par_to_star:
+  forall T T',
+  b_parr T T' -> b_star T T'.
+Proof.
+  intros T T' H. induction H.
+  - constructor.
+  - econstructor. constructor.
+    admit.
+  - admit.
+  - admit.
+Admitted.
 
